Source/DafnyStandardLibraries/examples/Actions/ActionsExamples.dfy
@@ -1,0 +1,177 @@
+module ActionsExamples {
+  import opened Std.Actions
+  import opened Std.Enumerators
+  import opened Std.Aggregators
+  import opened Std.Wrappers
+
+  class Box {
+    const i: nat
+
+    constructor(i: nat)
+      reads {}
+      ensures this.i == i
+    {
+      this.i := i;
+    }
+  }
+
+  function SeqRange(n: nat): seq<nat> {
+    seq(n, i => i)
+  }
+
+  lemma SeqRangeIncr(prefix: seq<nat>, n: nat)
+    requires prefix == SeqRange(n)
+    ensures prefix + [n] == SeqRange(n + 1)
+  {}
+
+  @AssumeCrossModuleTermination
+  class BoxEnumerator extends Action<(), Box> {
+
+    var nextValue: nat
+
+    ghost predicate Valid()
+      reads this, Repr
+      ensures Valid() ==> this in Repr
+      ensures Valid() ==> CanProduce(history)
+      decreases height, 0
+    {
+      && this in Repr
+      && CanProduce(history)
+      && nextValue == |history|
+    }
+
+    constructor()
+      ensures Valid()
+      ensures fresh(Repr)
+      ensures history == []
+    {
+      nextValue := 0;
+      history := [];
+      Repr := {this};
+      height := 1;
+    }
+
+    ghost predicate CanConsume(history: seq<((), Box)>, next: ())
+      decreases height
+    {
+      true
+    }
+    ghost predicate CanProduce(history: seq<((), Box)>)
+      decreases height
+    {
+      Seq.Map((b: Box) => b.i, Outputs(history)) == SeqRange(|history|)
+    }
+
+    method Invoke(t: ()) returns (r: Box)
+      requires Requires(t)
+      reads Reads(t)
+      modifies Modifies(t)
+      decreases Decreases(t).Ordinal()
+      ensures Ensures(t, r)
+    {
+      assert Requires(t);
+      ghost var producedBefore := Produced();
+
+      r := new Box(nextValue);
+      Update(t, r);
+      Repr := {this};
+      nextValue := nextValue + 1;
+
+      SeqRangeIncr(Seq.Map((b: Box) => b.i, producedBefore), |producedBefore|);
+      assert Valid();
+    }
+
+    method RepeatUntil(t: (), stop: Box -> bool, ghost eventuallyStopsProof: ProducesTerminatedProof<(), Box>)
+      requires Valid()
+      requires eventuallyStopsProof.Action() == this
+      requires eventuallyStopsProof.FixedInput() == t
+      requires eventuallyStopsProof.StopFn() == stop
+      requires forall i <- Consumed() :: i == t
+      reads Repr
+      modifies Repr
+      decreases Repr
+      ensures Valid()
+    {
+      DefaultRepeatUntil(this, t, stop, eventuallyStopsProof);
+    }
+  }
+
+  method {:rlimit 0} BoxEnumeratorExample() {
+    var enum: BoxEnumerator := new BoxEnumerator();
+    assert |enum.Produced()| == 0;
+    var a := enum.Invoke(());
+
+    assert enum.Produced() == [a];
+    assert Seq.Map((b: Box) => b.i, enum.Produced()) == SeqRange(1) == [0];
+    // assert a.i == 0;
+
+    // var b := enum.Invoke(());
+    // var c := enum.Invoke(());
+    // var d := enum.Invoke(());
+    // var e := enum.Invoke(());
+  }
+
+  method SetEnumeratorExample() {
+    var s: set<nat> := {1, 2, 3, 4, 5};
+    var copy: set<nat> := {};
+    var e: SetEnumerator<nat> := new SetEnumerator(s);
+
+    label before:
+    for enumerated := 0 to 5
+      invariant e.Valid()
+      invariant enumerated == |e.history|
+      invariant fresh(e.Repr - old@before(e.Repr))
+    {
+      var x := e.Invoke(());
+      copy := copy + {x};
+    }
+
+    // TODO: cool enough that we can statically invoke
+    // the enumerator the right number of times!
+    // But now prove that copy == s!
+    // assert |copy| == 5;
+    // assert copy == s;
+  }
+
+  method {:rlimit 0} AggregatorExample() {
+    var a: ArrayAggregator<nat> := new ArrayAggregator();
+    var _ := a.Invoke(1);
+    var _ := a.Invoke(2);
+    var _ := a.Invoke(3);
+    var _ := a.Invoke(4);
+    var _ := a.Invoke(5);
+    var _ := a.Invoke(6);
+    assert a.Consumed() == [1, 2, 3, 4, 5, 6];
+    assert a.storage.items == [1, 2, 3, 4, 5, 6];
+  }
+
+  @AssumeCrossModuleTermination
+  class ExamplePipeline<T> extends Pipeline<T, T> {
+    constructor(upstream: Enumerator<T>)
+      requires upstream.Valid()
+      ensures Valid()
+    {
+      this.upstream := upstream;
+      var buffer := new Collector<T>();
+
+      Repr := {this} + upstream.Repr + buffer.Repr;
+      history := [];
+      this.buffer := buffer;
+      this.height := upstream.height + buffer.height + 1;
+    }
+
+    method Process(u: Option<T>, a: Accumulator<T>)
+      requires a.Valid()
+      reads a.Repr
+      modifies a.Repr
+      ensures a.ValidAndDisjoint()
+    {
+      assert a.Valid();
+
+      if u.Some? {
+        a.CanConsumeAll(a.history, u.value);
+        a.Accept(u.value);
+      }
+    }
+  }
+}
